theories/typing/fixpoint.v
@@ -1,171 +1,115 @@
 From refinedc.typing Require Export type.
-From refinedc.typing Require Import programs bytes.
-From refinedc.typing Require Import exist constrained.
+From refinedc.typing Require Import programs exist constrained.
 Set Default Proof Using "Type*".
 Import uPred.
 
+Definition type_fixpoint_def `{!typeG Σ} {A} : ((A -> type) → (A -> type)) → (A → type) :=
+  λ T x, tyexists (λ ty, constrained (ty x) (⌜∀ x, ty x ⊑ T ty x⌝)).
+Definition type_fixpoint_aux : seal (@type_fixpoint_def). Proof. by eexists. Qed.
+Definition type_fixpoint := type_fixpoint_aux.(unseal).
+Global Arguments type_fixpoint {Σ _ A} _ _.
+Lemma type_fixpoint_unseal `{!typeG Σ} {A} : type_fixpoint = @type_fixpoint_def Σ _ A.
+Proof. rewrite -type_fixpoint_aux.(seal_eq) //. Qed.
 
 Section fixpoint.
-  Context `{!typeG Σ}.
+  Context `{!typeG Σ} {A : Type}.
+  Implicit Types (T : (A -> type) → (A -> type)).
 
-  (* TODO: Is it possible to use monotone fixpoints instead of guarded
-  fixpoints here? It is not obvious how to do that since the Iris
-  monotone fixpoint library is for BIs, not for OFEs. Maybe it could
-  work to make ty_own_val and ty_has_op_type trivial (as currently in
-  guarded)? This would be quite annoying as it would mean that
-  fixpoints are not movable. But maybe one can work around this
-  problem by unfolding the T once in the definition of the fixpoint
-  and making sure that the recursive occurence occurs under a pointer
-  such that it's ty_own is used which can be unfolded? I.e. something
-  like the following:
-
-   list_t_rec R := optional (&own R) null
-
-   list_t := list_t_rec (fixp R)
-
-  with ty_own (fixp R) β l ≡ ty_own (R (fixp R)) β l
-
-  Not sure if this would actually work, in particular if one can show
-  that fixp is a type. Maybe if one makes sharing trivial as well?
- *)
-(*
-  Inductive type_own_le (ty1 ty2 : type) : Prop :=
-    Type_own_le :
-      (∀ β l, ty1.(ty_own) β l -∗ ty2.(ty_own) β l) →
-      (∀ v, ty1.(ty_own_val) v -∗ ty2.(ty_own_val) v) →
-      type_own_le ty1 ty2.
-
-  Definition type_own_equiv (ty1 ty2 : type) : Prop :=
-    type_own_le ty1 ty2 ∧ type_own_le ty2 ty1.
-
-  Definition type_own_le_all {A} (ty1 ty2 : A → type) : Prop :=
-    ∀ x, type_own_le (ty1 x) (ty2 x).
-
-  Class TypeMono {A} (T : (A → type) → (A → type)) :=
-    type_mono ty1 ty2:
-      type_own_le_all ty1 ty2 →
-      type_own_le_all (T ty1) (T ty2).
-
-  Context {A : Type} (T : (A -> type) → (A -> type)).
-  Definition fixp : A → type :=
-    λ x, tyexists (λ ty, constrained (ty x) (⌜type_own_le_all ty (T ty)⌝)).
-
-  Lemma fixp_greatest ty :
-    type_own_le_all ty (T ty) →
-    type_own_le_all ty fixp.
+  Local Lemma type_fixpoint_own_eq T x l β :
+    l ◁ₗ{β} type_fixpoint T x ⊣⊢ ∃ ty, ⌜∀ x, ty x ⊑ T ty x⌝ ∗ l ◁ₗ{β} ty x.
   Proof.
-    move => Hle.
-    split.
-    - iIntros (β l) "Hl". rewrite {2}/ty_own/=. iExists _.
-      rewrite tyexists_eq. rewrite /own_constrained/={2}/ty_own/=/persistent_own_constraint. iFrame.
-      iPureIntro. done.
-    - iIntros (v) "Hv". rewrite {2}/ty_own_val/=. iExists _.
-      rewrite tyexists_eq. rewrite /own_constrained/={2}/ty_own_val/=/persistent_own_constraint. iFrame.
-      iPureIntro. done.
+    rewrite type_fixpoint_unseal {1}/ty_own/=. f_equiv => ?.
+    rewrite tyexists_eq. rewrite /own_constrained/persistent_own_constraint; simpl_type.
+    iSplit; by iIntros "[$ ?]".
   Qed.
 
-  Lemma fixp_unfold_1 `{!TypeMono T}:
-    type_own_le_all fixp (T fixp).
+  Local Lemma type_fixpoint_own_val_eq T x v :
+    v ◁ᵥ type_fixpoint T x ⊣⊢ ∃ ty, ⌜∀ x, ty x ⊑ T ty x⌝ ∗ v ◁ᵥ ty x.
   Proof.
-    intros x. split; simpl.
-    - iIntros (??) "[%ty HA]". simpl in *. rewrite tyexists_eq.
-      rewrite /own_constrained/={1}/ty_own/=/persistent_own_constraint.
-      iDestruct "HA" as "[HA %Hle]".
-      move: (Hle) => Hle2.
-      destruct (Hle2 x) as [Hown ?].
-      iDestruct (Hown with "HA") as "HA".
-      edestruct (type_mono ty fixp) as [Hown2 ?]; [|by iApply Hown2].
-      intros. by apply fixp_greatest.
-    - iIntros (?) "[%ty HA]". simpl in *. rewrite tyexists_eq.
-      rewrite /own_constrained/={1}/ty_own_val/=/persistent_own_constraint.
-      iDestruct "HA" as "[HA %Hle]".
-      move: (Hle) => Hle2.
-      destruct (Hle2 x) as [? Hown].
-      iDestruct (Hown with "HA") as "HA".
-      edestruct (type_mono ty fixp) as [? Hown2]; [|by iApply Hown2].
-      intros. by apply fixp_greatest.
+    rewrite type_fixpoint_unseal {1}/ty_own_val/=. f_equiv => ?.
+    rewrite tyexists_eq. rewrite /own_constrained/persistent_own_constraint; simpl_type.
+    iSplit; by iIntros "[$ ?]".
   Qed.
 
-  Lemma fixp_unfold_2 `{!TypeMono T} :
-    type_own_le_all (T fixp) fixp.
+  Lemma type_fixpoint_greatest T ty :
+    (∀ x, ty x ⊑ T ty x) →
+    ∀ x, ty x ⊑ type_fixpoint T x.
   Proof.
-    intros x. split; simpl.
-    - iIntros (??) "?". iExists _. rewrite tyexists_eq.
-      rewrite /own_constrained/={2}/ty_own/=/persistent_own_constraint. iSplit; [done|].
-      iPureIntro. intros. apply type_mono. intros. by apply fixp_unfold_1.
-    - iIntros (?) "?". iExists _. rewrite tyexists_eq.
-      rewrite /own_constrained/={2}/ty_own_val/=/persistent_own_constraint. iFrame.
-      iPureIntro. intros. apply type_mono. intros. by apply fixp_unfold_1.
+    move => Hle. constructor.
+    - iIntros (β l) "Hl". rewrite type_fixpoint_own_eq. iExists _. by iFrame.
+    - iIntros (v) "Hv". rewrite type_fixpoint_own_val_eq. iExists _. by iFrame.
   Qed.
 
-  Lemma fixp_unfold x `{!TypeMono T} :
-    type_own_equiv (fixp x) (T fixp x).
-  Proof. split; [by apply fixp_unfold_1 | by apply fixp_unfold_2]. Qed.
-
-  Lemma fixp_unfold2 x `{!TypeMono T}:
-    type_own_equiv (T fixp x) (T (T fixp) x).
-  Proof. split; apply type_mono; intros ?; by apply fixp_unfold. Qed.
-*)
-
-  Global Instance type_inhabited : Inhabited type := populate (uninit void_layout).
-
-  Context {A : Type} (T : (A -d> typeO) → (A -d> typeO)) {HT: Contractive T}.
-
-  Definition type_fixpoint : (A -d> typeO) → (A -d> typeO) := (λ self, T (λ x, apply_dfun self x)).
-  Global Instance type_fixpoint_contractive : Contractive type_fixpoint.
+  Lemma type_fixpoint_unfold_1 T `{!TypeMono T}:
+    ∀ x, type_fixpoint T x ⊑ T (type_fixpoint T) x.
   Proof.
-    constructor; intros.
-    - eapply ty_has_op_type_ne => //. apply HT. solve_contractive.
-    - apply ty_own_ne => //. apply HT. solve_contractive.
-    - apply ty_own_val_ne => //. apply HT. solve_contractive.
+    intros x. constructor => *.
+    - rewrite type_fixpoint_own_eq. iIntros "[%ty [%Hle HA]]".
+      destruct (Hle x) as [-> ?].
+      edestruct (TypeMono0 ty (type_fixpoint T)) as [Hown2 ?]; [|by iApply Hown2].
+      intros ?. by apply type_fixpoint_greatest.
+    - rewrite type_fixpoint_own_val_eq. iIntros "[%ty [%Hle HA]]".
+      destruct (Hle x) as [? ->].
+      edestruct (TypeMono0 ty (type_fixpoint T)) as [? Hown2]; [|by iApply Hown2].
+      intros ?. by apply type_fixpoint_greatest.
   Qed.
 
+  Lemma type_fixpoint_unfold_2 T `{!TypeMono T} :
+    ∀ x, T (type_fixpoint T) x ⊑ type_fixpoint T x.
+  Proof.
+    intros x. constructor => *.
+    - rewrite type_fixpoint_own_eq. iIntros "?". iExists _. iSplit; [|done].
+      iPureIntro. intros. apply TypeMono0. intros ?. by apply type_fixpoint_unfold_1.
+    - rewrite type_fixpoint_own_val_eq. iIntros "?". iExists _. iSplit; [|done].
+      iPureIntro. intros. apply TypeMono0. intros ?. by apply type_fixpoint_unfold_1.
+  Qed.
 
-  Definition fixp := (apply_dfun (fixpoint type_fixpoint)).
+  Lemma type_fixpoint_unfold T x `{!TypeMono T} :
+    type_fixpoint T x ≡ T (type_fixpoint T) x.
+  Proof. apply (anti_symm (⊑)); [by apply type_fixpoint_unfold_1 | by apply type_fixpoint_unfold_2]. Qed.
 
-  Lemma fixp_unfold n:
-    fixp n ≡ T (λ n, fixp n) n.
-  Proof. rewrite /fixp. rewrite ->fixpoint_unfold. rewrite /apply_dfun{1}/type_fixpoint. f_equiv. Qed.
-
-  Lemma fixp_unfold' x:
-    T fixp x ≡@{type} T (T fixp) x.
-  Proof. apply (contractive_proper T) => ?. by rewrite -fixp_unfold. Qed.
+  Lemma type_fixpoint_unfold2 T x `{!TypeMono T}:
+    T (type_fixpoint T) x ≡ T (T (type_fixpoint T)) x.
+  Proof.
+    apply (anti_symm (⊑)); apply TypeMono0;
+      intros ?; [by apply type_fixpoint_unfold_1 | by apply type_fixpoint_unfold_2].
+  Qed.
 End fixpoint.
 
 Section fixpoint.
   Context `{!typeG Σ}.
-  Lemma fixp_proper {A} x1 x2 (T1 T2 : (A -d> typeO) → (A -d> typeO)) `{!Contractive T1} `{!Contractive T2}:
+
+  Lemma type_fixpoint_proper {A} x1 x2 (T1 T2 : (A → type) → (A → type)) :
     x1 = x2 → (∀ f x, T1 f x ≡ T2 f x) →
-    fixp T1 x1 ≡ fixp T2 x2.
+    type_fixpoint T1 x1 ≡ type_fixpoint T2 x2.
   Proof.
-    move => ? HT. rewrite /fixp.
-    apply apply_dfun_proper => //.
-    apply fixpoint_proper => ?.
-    rewrite /type_fixpoint.
-    apply: HT.
+    move => -> HT.
+    constructor => *.
+    - rewrite !type_fixpoint_own_eq. by setoid_rewrite HT.
+    - rewrite !type_fixpoint_own_val_eq. by setoid_rewrite HT.
   Qed.
 End fixpoint.
 
 (*** Tests *)
 Section tests.
   Context `{!typeG Σ}.
-  Context (own_ptr : type → type) {HT: NonExpansive own_ptr}.
+  Context (own_ptr : type → type) {HT: Proper ((⊑) ==> (⊑)) own_ptr}.
 
-  Definition fixpoint_test_rec : (nat -d> typeO) → (nat -d> typeO) := (λ self, λ n, own_ptr (guarded ("test") (apply_dfun self (S n)))).
+  Definition fixpoint_test_rec : (nat → type) → (nat → type) := (λ self, λ n, own_ptr (self (S n))).
   Arguments fixpoint_test_rec /.
-  Global Instance fixpoint_test_rec_ne : Contractive fixpoint_test_rec.
+  Global Instance fixpoint_test_rec_ne : TypeMono fixpoint_test_rec.
   Proof. solve_type_proper. Qed.
 
   Definition fixpoint_test : rtype := {|
     rty_type := nat;
-    rty n := fixp fixpoint_test_rec n
+    rty n := type_fixpoint fixpoint_test_rec n
   |}.
 
   Example test l :
     l◁ₗ 0%nat @ fixpoint_test -∗ True.
   Proof.
-    simpl. rewrite /with_refinement/= fixp_unfold/apply_dfun/=.
-    change (fixp _ _) with (1%nat @ fixpoint_test)%I.
+    simpl. rewrite /with_refinement/= type_fixpoint_unfold/=.
+    change (type_fixpoint _ _) with (1%nat @ fixpoint_test)%I.
   Abort.
 
 End tests.
